src/Examples/Logging2/Log2API.v
@@ -20,10 +20,8 @@ Module Log2.
          match op with
          | Append l' =>
             curl <- reads (fun l => l);
-            if gt_dec (length curl + length l') log_size then
-              pure false
-            else
-              _ <- puts (fun l => l ++ l'); pure true
+            ( pure false ) + 
+            ( _ <- puts (fun l => l ++ l'); pure true )
          | Read => reads (fun l => l)
          end;
        crash_step := pure tt;
